Foundation/Propositional/Classical/Hilbert.lean
@@ -1,0 +1,93 @@
+import Foundation.Propositional.Hilbert.WellKnown
+import Foundation.Propositional.Classical.Basic
+import Foundation.Propositional.ConsistentTableau
+
+namespace LO.Propositional
+
+namespace Hilbert.Cl.Classical
+
+-- Semantics.Valid (Classical.Valuation ℕ) φ
+lemma soundness (h : Hilbert.Cl ⊢! φ) : ∀ v, φ.val v := by
+  induction h using Hilbert.Deduction.rec! with
+  | maxm h =>
+    rcases h with ⟨φ, (rfl | rfl), ⟨_, rfl⟩⟩ <;> { intro v; tauto; }
+  | mdp ihφψ ihφ => intro v; exact ihφψ v $ ihφ v;
+  | orElim => simp [Formula.val]; tauto;
+  | _ => simp_all [Formula.val];
+
+
+section
+
+open
+  Entailment
+  SaturatedConsistentTableau
+
+def canonicalVal (T : SaturatedConsistentTableau Hilbert.Cl) : Classical.Valuation ℕ where
+  val a := (.atom a) ∈ T.1.1
+
+lemma truthlemma {T : SaturatedConsistentTableau Hilbert.Cl} : φ.val (canonicalVal T) ↔ φ ∈ T.1.1 := by
+  induction φ using Formula.rec' with
+  | hatom => simp [Formula.val, canonicalVal];
+  | hfalsum => simp [Formula.val, canonicalVal];
+  | himp φ ψ ihφ ihψ =>
+    constructor;
+    . intro hφψ;
+      rcases imp_iff_not_or.mp hφψ with hφ | hψ;
+      . apply iff_mem₁_imp.mpr;
+        left;
+        exact iff_not_mem₁_mem₂.mp $ ihφ.not.mp $ hφ;
+      . apply iff_mem₁_imp.mpr;
+        right;
+        exact ihψ.mp hψ;
+    . rintro hφψ hφ;
+      apply ihψ.mpr;
+      rcases iff_mem₁_imp.mp hφψ with hφ | hψ;
+      . have := ihφ.not.mpr $ iff_not_mem₁_mem₂.mpr hφ; contradiction;
+      . exact hψ;
+  | hand φ ψ ihφ ihψ =>
+    constructor;
+    . rintro ⟨hφ, hψ⟩;
+      apply iff_mem₁_and.mpr;
+      constructor;
+      . apply ihφ.mp hφ;
+      . apply ihψ.mp hψ;
+    . rintro hφψ;
+      rcases iff_mem₁_and.mp hφψ with ⟨hφ, hψ⟩;
+      constructor;
+      . apply ihφ.mpr hφ;
+      . apply ihψ.mpr hψ;
+  | hor φ ψ ihφ ihψ =>
+    constructor;
+    . rintro (hφ | hψ);
+      . apply iff_mem₁_or.mpr;
+        left;
+        apply ihφ.mp hφ;
+      . apply iff_mem₁_or.mpr;
+        right;
+        apply ihψ.mp hψ;
+    . rintro hφψ;
+      rcases iff_mem₁_or.mp hφψ with hφ | hψ;
+      . left; apply ihφ.mpr hφ;
+      . right; apply ihψ.mpr hψ;
+
+lemma completeness : (∀ v, φ.val v) → (Hilbert.Cl ⊢! φ) := by
+  contrapose;
+  intro h;
+  push_neg;
+  obtain ⟨T, hT⟩ := lindenbaum (𝓢 := Hilbert.Cl) (t₀ := (∅, {φ})) $ by
+    intro Γ Δ hΓ hΔ;
+    by_contra hC;
+    replace hΓ : Γ = [] := List.eq_nil_iff_forall_not_mem.mpr hΓ;
+    subst hΓ;
+    exact h $ disj_allsame'! hΔ (hC ⨀ verum!);
+  use (canonicalVal T);
+  apply truthlemma.not.mpr;
+  apply iff_not_mem₁_mem₂.mpr;
+  apply hT.2;
+  tauto;
+
+end
+
+end Hilbert.Cl.Classical
+
+end LO.Propositional
